proof.v
@@ -2,44 +2,18 @@ Require Import Local.subterm.
 Require Import MetaCoq.Template.All.
 Require Import MetaCoq.Checker.All.
 Require Import String.
+Require Import Arith.Wf_nat.
 
 Require Import List.
 Import ListNotations.
 
 Ltac inj H := (injection H; clear H; intro H).
 
-Lemma ind_inversion:
-  forall Sigma mind_body ind,
-  wf (Sigma) ->
-  declared_minductive (Sigma) (inductive_mind ind) mind_body ->
-  let u := universes_decl_of_decl
-            (InductiveDecl (inductive_mind ind) mind_body)
-  in
-  on_inductive (lift_typing typing)
-               (Sigma, u)
-               (inductive_mind ind) mind_body.
-Proof.
-  intros Sigma mind_body ind W D u.
-  induction W.
-  - inversion D.
-  - destruct (ident_eq (inductive_mind ind) (global_decl_ident d)) eqn: e;
-    unfold declared_minductive in D; cbn in D; rewrite e in D.
-    + inj D. subst.
-      change (on_global_decl (lift_typing typing) (Σ,, InductiveDecl (inductive_mind ind) mind_body, u) (InductiveDecl (inductive_mind ind) mind_body)).
-      apply (WeakeningEnv.weakening_on_global_decl (lift_typing typing) Σ _ _ (InductiveDecl (inductive_mind ind) mind_body)).
-      exact WeakeningEnv.weaken_env_prop_typing.
-      constructor; assumption. exists [InductiveDecl (inductive_mind ind) mind_body]. reflexivity. assumption.
-    + unfold declared_minductive in IHW. apply IHW in D.
-      change (on_global_decl (lift_typing typing) (Σ,, d, u) (InductiveDecl (inductive_mind ind) mind_body)).
-      apply (WeakeningEnv.weakening_on_global_decl (lift_typing typing) Σ _ _ (InductiveDecl (inductive_mind ind) mind_body)).
-      exact WeakeningEnv.weaken_env_prop_typing.
-      constructor; assumption. exists [d]. reflexivity. assumption.
-Qed.
-
-Lemma decompose_it_mkProd l m:
-  forall c s, (forall n, (c ++ n, s) = decompose_prod_assum n m) ->
+Lemma decompose_it_mkProd l m c s:
+  (forall n, (c ++ n, s) = decompose_prod_assum n m) ->
   decompose_prod_assum [] (it_mkProd_or_LetIn l m) = (c ++ l, s).
 Proof.
+  generalize c s. clear c s.
   induction l in m |- *; intros c s e; cbn.
   - specialize e with []. rewrite app_nil_r in e. now rewrite app_nil_r.
   - cbn. change ((fold_left (fun acc d => mkProd_or_LetIn d acc) l (mkProd_or_LetIn a m))) with (it_mkProd_or_LetIn l (mkProd_or_LetIn a m)).
@@ -73,29 +47,92 @@ Lemma it_mkProd_assoc a b c:
   it_mkProd_or_LetIn b (it_mkProd_or_LetIn a c) = it_mkProd_or_LetIn (a ++ b) c.
 Proof. induction a in b, c |- *; cbn; auto. Qed.
 
-Goal forall Sigma mind_body ref ind,
-    wf Sigma ->
-    {u & ref = tInd ind u} ->
+Lemma rev_list_ind_t {A} : forall P:list A-> Type,
+  P [] ->
+  (forall (a:A) (l:list A), P (rev l) -> P (rev (a :: l))) ->
+  forall l:list A, P (rev l).
+Proof.
+  induction l; auto.
+Qed.
+
+Theorem rev_ind_t {A} : forall P:list A -> Type,
+  P [] ->
+  (forall (x:A) (l:list A), P l -> P (l ++ [x])) -> forall l:list A, P l.
+Proof.
+  intros.
+  generalize (rev_involutive l).
+  intros E; rewrite <- E.
+  apply (rev_list_ind_t P).
+  - auto.
+  - simpl. intros. apply (X0 a (rev l0)). auto.
+Qed.
+
+Lemma type_type {Sigma} {Gamma} {u} {t} {T}:
+  (Sigma, u);;; Gamma |- t : T ->
+  {s & (Sigma, u);;; Gamma |- T : tSort s}.
+Proof.
+  intros.
+  induction X.
+  - assert (n < #|Γ|) as lenG. (now apply nth_error_Some).
+    pose (nth_error_All_local_env lenG a).
+    admit.
+  - induction l; cbn.
+    
+Admitted.
+
+
+Lemma it_mkProd_typed {Sigma} {Gamma} {u} {l} {r} {s}:
+  (Sigma, u);;; (l ++ Gamma) |- r : tSort s ->
+  {s & (Sigma, u);;; Gamma |- it_mkProd_or_LetIn l r : tSort s}.
+Proof.
+  revert r s.
+  induction l; intros.
+  - eauto using app_nil_r, X.
+  - simpl.
+    assert ({s1 & (Sigma, u);;; (l ++ Gamma) |- mkProd_or_LetIn a r : tSort s1}).
+    destruct a eqn: eqa.
+    destruct decl_body.
+    assert (0 < #|(a :: l) ++ Gamma|) as lenG; simpl; try micromega.Lia.lia.
+    subst. pose (nth_error_All_local_env lenG (typing_wf_local X)) as o.
+    cbn in o. try destruct o as [eo o].
+    unfold mkProd_or_LetIn. simpl.
+    destruct (type_type o). eexists.
+    apply (type_Conv _ _ _ (tLetIn decl_name t decl_type (tSort s)) _).
+    eapply type_LetIn. exact t0. exact o. unfold vdef, snoc. exact X.
+    unfold isWfArity. right. eexists. apply type_Sort.
+    exact (typing_wf_local o).
+    inversion o.
+    + admit.
+Admitted.
+
+Goal forall Sigma mind_body ref ind u,
+    wf_ext Sigma ->
+    ref = tInd ind u ->
+(*    consistent_instance_ext Sigma mind_body.(ind_universes) u ->*)
     declared_minductive (Sigma) (inductive_mind ind) mind_body ->
     forall v, direct_subterm_for_mutual_ind mind_body ind ref = Some v ->
-    wf (Sigma ,, InductiveDecl ("random"%string) v).
+    wf (Sigma.1 ,, ("random"%string, InductiveDecl  v)).
 Proof.
-  intros Sigma mind_body ref ind WF EU DM v Sv.
-  pose (Monomorphic_ctx (LevelSet.empty, ConstraintSet.empty)) as ctx.
+  intros Sigma mind_body ref ind ui WF EtInd (*CUI*) DM v Sv.
+  destruct WF as [WF WFU].
   constructor.
   - inversion WF; constructor; try assumption.
   - admit.
-  - admit.
-  - constructor; unfold direct_subterm_for_mutual_ind in Sv;
+  - unfold direct_subterm_for_mutual_ind in Sv.
     destruct (nth_error (ind_bodies mind_body) (inductive_ind ind)) eqn: ind_body; cbn in Sv.
-    2:congruence. inj Sv.
-    + destruct (ind_inversion Sigma mind_body ind WF DM).
-      rewrite <- Sv; constructor.
-      pose (universes_decl_of_decl
-              (InductiveDecl (inductive_mind ind) mind_body)) as u.
+    inj Sv. 2 : congruence.
+    destruct (WeakeningEnv.on_declared_minductive WF DM).
+    rewrite <- Sv. cbn. admit.
+  - unfold direct_subterm_for_mutual_ind in Sv.
+    destruct (nth_error (ind_bodies mind_body) (inductive_ind ind)) eqn: ind_body; cbn in Sv.
+    inj Sv. 2 : congruence.
+    constructor;
+    destruct (WeakeningEnv.on_declared_minductive WF DM).
+    + rewrite <- Sv; constructor.
+      pose (ind_universes mind_body) as u.
       destruct (Alli_nth_error
                   (on_ind_body (lift_typing typing)
-                               (Sigma, u)
+                               (Sigma.1, u)
                                (inductive_mind ind) mind_body)
                   0 _ onInductives _ o ind_body).
       2: constructor. eapply (Build_on_ind_body _ _ _ _ _ _ _ _).
@@ -111,21 +148,65 @@ Proof.
         rewrite ind_arity_eq.
         destruct decompose_prod_assum eqn: decomp_eq.
 
-        rewrite it_mkProd_assoc. exists (Universe.make' (Level.lProp, false)).
+        rewrite it_mkProd_assoc. cbn.
+        eexists.
+        (*exists (Universe.make' (Level.lProp, false)).*)
         rewrite it_mkProd_assoc in decomp_eq.
         erewrite decompose_it_mkProd in decomp_eq.
 
-        Focus 2. intro. (* ?c *) Existential 13 := []. reflexivity.
+        Focus 2. intro. (* ?c *) Existential 11 := []. reflexivity.
+
         rewrite app_nil_l in decomp_eq.
         inversion decomp_eq.
-        rewrite app_length, PeanoNat.Nat.add_sub, firstn_app, PeanoNat.Nat.sub_diag, firstn_all, app_nil_r. cbn. admit.
-      * admit.
-      * intros. unfold subterm_for_ind in H. unfold ind_projs in H. destruct (decompose_prod_assum [] (ind_type o)). now contradiction H.
-      * cbn. intros x H. unfold subterm_for_ind in H. unfold ind_kelim in H.
-        destruct (decompose_prod_assum [] (ind_type o)).
-        induction H. rewrite <- H. now cbn. inversion H.
-      Unshelve.
-    + cbn. constructor.
-Abort.
+        rewrite app_length, PeanoNat.Nat.add_sub, firstn_app,
+                PeanoNat.Nat.sub_diag, firstn_all, app_nil_r, <- it_mkProd_assoc.
+        cbn in onParams. cbn. admit.
+      * unfold on_udecl_decl. cbn.
+        rewrite Sv.
 
+        unfold ind_ctors.
+        unfold subterm_for_ind at 2.
+        destruct decompose_prod_assum eqn: decomp_eq.
+        destruct o eqn: eqo. unfold Ast.ind_ctors.
+        unfold mapi. generalize 0.
+        unfold on_constructors. simpl in onConstructors.
+        clear ind_sorts.
+        induction onConstructors as [ | a b l m onAB onLM IH]; intro n.
+        -- (* MetaCoq 8.11 broke this *)
+           (*simpl. unfold on_constructors. apply All2_nil.*)
+           admit.
+        -- unfold mapi. rewrite mapi_rec_eqn.
+           destruct a. destruct p.
+           rewrite concat_cons.
+           set (tail n := (concat (mapi_rec (fun (n1 : nat) '(id', ct, k) => map
+             (fun '(si, st, sk) =>
+              ((id' ++ "_subterm" ++ string_of_nat si)%string, st, sk))
+             (subterms_for_constructor ind ref #|ind_bodies mind_body|
+                #|ind_params mind_body|
+                #|firstn (#|c| - #|ind_params mind_body|) c| ct n1 k))
+                                           l  n))).
+           fold (tail (S n)). fold (tail n) in IH.
+           unfold subterms_for_constructor at 1.
 
+           destruct (decompose_prod_assum [] t0) as [ca cs] eqn: cteq.
+           unfold on_constructor, on_type in onAB.
+           inversion onAB as [onAB_type [[cons_args cons_concl_head cons_inds cons_eq] WTlocal]].
+           simpl in cshape_eq. rewrite cshape_eq in cteq.
+           rewrite it_mkProd_assoc in cteq.
+           rewrite (decompose_it_mkProd _ _
+                                        []
+                                        (mkApps cons_inds (to_extended_list_k (ind_params mind_body) #|cons_args| ++ cons_eq)))
+             in cteq.
+           Focus 2.
+           set (ll := (to_extended_list_k (ind_params mind_body) #|cons_args| ++ cons_eq)).
+           destruct ll eqn: ll_eq; simpl; reflexivity.
+           inversion cteq.
+           admit.
+      * intros. unfold subterm_for_ind in H. unfold ind_projs in H.
+        destruct (decompose_prod_assum [] (ind_type o)). now contradiction H.
+      * cbn. unfold ind_kelim, subterm_for_ind.
+        now destruct (decompose_prod_assum [] (ind_type o)); cbn.
+    + subst. now constructor.
+    + subst. now simpl.
+    + (* ind_guard - just assume that it holds?*) admit.
+Admitted.
